progress on proving memory safety

code/experimental/rsa/Hacl.Impl.Exponentiation.fst
@@ -14,24 +14,26 @@ module Buffer = Spec.Lib.IntBuf
 
 val mul_mod_mont:
   #rLen:size_nat -> rrLen:size_t{v rrLen == rLen /\ rLen + rLen < max_size_t} ->
-  pow2_i:size_t{2 * rLen + 4 * v pow2_i < max_size_t /\ rLen < v pow2_i} -> 
+  pow2_i:size_t{2 * rLen + 4 * v pow2_i < max_size_t /\ rLen < v pow2_i} ->
   iLen:size_t{v iLen < v pow2_i / 2 /\ v iLen + rLen = v pow2_i} ->
   n:lbignum rLen -> nInv_u64:uint64 -> st_kara:lbignum (2 * rLen + 4 * v pow2_i) ->
   aM:lbignum rLen -> bM:lbignum rLen -> resM:lbignum rLen ->
   Stack unit
-    (requires (fun h -> live h aM /\ live h bM /\ live h resM /\ live h n /\ live h st_kara))
-    (ensures (fun h0 _ h1 -> preserves_live h0 h1))
+    (requires (fun h -> live h aM /\ live h bM /\ live h resM /\ live h n /\ live h st_kara /\
+                      disjoint st_kara aM /\ disjoint st_kara bM /\ disjoint st_kara n))
+    (ensures (fun h0 _ h1 -> preserves_live h0 h1 /\ modifies2 resM st_kara h0 h1))
   [@"c_inline"]
 let mul_mod_mont #rLen rrLen pow2_i iLen n nInv_u64 st_kara aM bM resM =
   let cLen = add #SIZE rrLen rrLen in
   let stLen = add #SIZE cLen (mul #SIZE (size 4) pow2_i) in
-  
   let c = Buffer.sub #uint64 #(v stLen) #(v cLen) st_kara (size 0) cLen in
-  let st_kara' = Buffer.sub #uint64 #(v stLen) #(4 * v pow2_i) st_kara cLen (mul #SIZE (size 4) pow2_i) in
-  assume (disjoint c aM /\ disjoint c bM /\ disjoint st_kara' aM /\ disjoint st_kara' bM);
-  karatsuba pow2_i iLen rrLen aM bM st_kara' c; // c = aM * bM
   assume (disjoint c n);
-  mont_reduction rrLen n nInv_u64 c c resM // resM = c % n
+  
+  karatsuba pow2_i iLen rrLen aM bM st_kara; // c = aM * bM
+  let h0 = FStar.HyperStack.ST.get() in
+  mont_reduction rrLen n nInv_u64 c c resM; // resM = c % n 
+  let h1 = FStar.HyperStack.ST.get() in
+  assume (modifies2 resM st_kara h0 h1)
 
 val mod_exp_:
   #rLen:size_nat -> rrLen:size_t{v rrLen == rLen /\ rLen + rLen < max_size_t} ->
@@ -41,19 +43,21 @@ val mod_exp_:
   bBits:size_t{0 < v bBits} -> bLen:size_t{v bLen = v (bits_to_bn bBits) /\ v bBits / 64 < v bLen} -> b:lbignum (v bLen) ->
   i:size_t{v i <= v bBits} ->
   Stack unit
-    (requires (fun h -> live h n /\ live h b /\ live h st_kara /\ live h st_exp))
-    (ensures  (fun h0 _ h1 -> preserves_live h0 h1))
+    (requires (fun h -> live h n /\ live h b /\ live h st_kara /\ live h st_exp /\
+                      disjoint st_exp st_kara /\ disjoint st_kara n))    
+    (ensures  (fun h0 _ h1 -> preserves_live h0 h1 /\ modifies2 st_exp st_kara h0 h1))
   [@"c_inline"]
 let rec mod_exp_ #rLen rrLen pow2_i iLen n nInv_u64 st_kara st_exp bBits bLen b i =
   let aM = Buffer.sub #uint64 #(rLen + rLen) #rLen st_exp (size 0) rrLen in
   let accM = Buffer.sub #uint64 #(rLen + rLen) #rLen st_exp rrLen rrLen in
-  
-  if (i <. bBits) then begin
+  disjoint_sub_lemma1 st_exp st_kara (size 0) rrLen; // disjoint st_kara aM
+  disjoint_sub_lemma1 st_exp st_kara rrLen rrLen; // disjoint st_kara accM
+  (if (i <. bBits) then begin
     (if (bn_is_bit_set bLen b i) then mul_mod_mont rrLen pow2_i iLen n nInv_u64 st_kara aM accM accM); // acc = (acc * a) % n
     mul_mod_mont rrLen pow2_i iLen n nInv_u64 st_kara aM aM aM; // a = (a * a) % n
     mod_exp_ rrLen pow2_i iLen n nInv_u64 st_kara st_exp bBits bLen b (size_incr i)
-  end
-
+  end); admit()
+  
 
 val mod_exp_mont:
   #rLen:size_nat -> rrLen:size_t{v rrLen == rLen /\ rLen + rLen < max_size_t} ->
@@ -63,7 +67,7 @@ val mod_exp_mont:
   nInv_u64:uint64 -> st:lbignum (9 * rLen + 4 * v pow2_i) ->
   Stack unit
     (requires (fun h -> live h b /\ live h st))
-    (ensures  (fun h0 _ h1 -> preserves_live h0 h1))
+    (ensures  (fun h0 _ h1 -> preserves_live h0 h1 /\ modifies1 st h0 h1))
   #reset-options "--z3rlimit 150 --max_fuel 0"
   [@"c_inline"]
 let mod_exp_mont #rLen rrLen pow2_i iLen bBits b nInv_u64 st =
@@ -88,7 +92,7 @@ let mod_exp_mont #rLen rrLen pow2_i iLen bBits b nInv_u64 st =
   to_mont rrLen pow2_i iLen n1 nInv_u64 r2 a1 st_kara aM;
   to_mont rrLen pow2_i iLen n1 nInv_u64 r2 acc st_kara accM;
   mod_exp_ rrLen pow2_i iLen n1 nInv_u64 st_kara st_exp bBits bLen b (size 0);
-  from_mont rrLen pow2_i iLen n1 nInv_u64 accM st' res1
+  from_mont rrLen pow2_i iLen n1 nInv_u64 accM st' res1; admit()
 
 // res = a ^^ b mod n
 val mod_exp:
@@ -100,11 +104,11 @@ val mod_exp:
   bBits:size_t{0 < v bBits} -> b:lbignum (v (bits_to_bn bBits)) -> res:lbignum nLen ->
   Stack unit
     (requires (fun h -> live h n /\ live h a /\ live h b /\ live h res))
-    (ensures  (fun h0 _ h1 -> preserves_live h0 h1))
+    (ensures  (fun h0 _ h1 -> preserves_live h0 h1 /\ modifies1 res h0 h1))
   #reset-options "--z3rlimit 150 --max_fuel 0"
   [@"c_inline"]    
 let mod_exp #nLen pow2_i iLen modBits nnLen n a bBits b res =
-  push_frame();
+  //push_frame();
   let rrLen = size_incr nnLen in
   assume (128 * v rrLen < max_size_t);
   let exp_r = mul #SIZE (size 64) rrLen in
@@ -140,7 +144,6 @@ let mod_exp #nLen pow2_i iLen modBits nnLen n a bBits b res =
     let nInv_u64 = mod_inv_u64 n0 in // n * nInv = 1 (mod (pow2 64))
     mod_exp_mont #(v rrLen) rrLen pow2_i iLen bBits b nInv_u64 st;
       
-    copy nnLen res1' res;
-    admit()
-    );
-    pop_frame()
+    copy nnLen res1' res
+    )
+    //pop_frame()
