code/experimental/rsa/Hacl.Impl.Montgomery.fst
@@ -69,19 +69,39 @@ let mod_inv_u64 n0 =
   let vb = u64 0 in
   mod_inv_u64_ alpha beta ub vb (size 0)
 
+val bn_mult_by_limb_addj_carry:
+  #aLen:size_nat -> aaLen:size_t{v aaLen == aLen} -> a:lbignum aLen ->
+  l:uint64 -> carry:uint64 -> i:size_t{v i <= aLen} -> j:size_t ->
+  resLen:size_t{aLen + v j < v resLen} -> res:lbignum (v resLen) -> Stack uint64
+  (requires (fun h -> live h a /\ live h res /\ disjoint res a))
+  (ensures (fun h0 _ h1 -> preserves_live h0 h1 /\ modifies1 res h0 h1))
+  [@"c_inline"]
+let rec bn_mult_by_limb_addj_carry #aLen aaLen a l carry i j resLen res =
+  let ij = add #SIZE i j in
+  if (i <. aaLen) then begin
+    let res_ij = res.(ij) in
+    let (carry', res_ij) = bn_mul_by_limb_addj_f a.(i) l carry res_ij in
+    res.(ij) <- res_ij;
+    bn_mult_by_limb_addj_carry aaLen a l carry' (size_incr i) j resLen res end
+  else begin
+    let res_ij = res.(ij) in
+    let (c', res_ij) = addcarry_u64 (u64 0) res_ij carry in
+    res.(ij) <- res_ij;
+    c' end
+      
 val mont_reduction_:
   #rLen:size_nat -> rrLen:size_t{v rrLen == rLen /\ rLen + rLen < max_size_t} ->
-  c:lbignum (rLen + rLen) -> n:lbignum rLen -> nInv_u64:uint64 -> i:size_t -> 
-  Stack unit
+  c:lbignum (rLen + rLen) -> n:lbignum rLen -> nInv_u64:uint64 ->
+  i:size_t -> carry':uint64 -> Stack unit
     (requires (fun h -> live h c /\ live h n /\ disjoint c n))
     (ensures (fun h0 _ h1 -> preserves_live h0 h1 /\ modifies1 c h0 h1))
   [@"c_inline"]
-let rec mont_reduction_ #rLen rrLen c n nInv_u64 i =
+let rec mont_reduction_ #rLen rrLen c n nInv_u64 i carry' =
   if (i <. rrLen) then begin
     let ci = c.(i) in
     let qi = mul_mod #U64 nInv_u64 ci in
-    bn_mult_by_limb_addj rrLen n qi (size 0) i (add #SIZE rrLen rrLen) (u64 0) c;
-    mont_reduction_ rrLen c n nInv_u64 (size_incr i)
+    let carry' = bn_mult_by_limb_addj_carry rrLen n qi carry' (size 0) i (add #SIZE rrLen rrLen) c in
+    mont_reduction_ rrLen c n nInv_u64 (size_incr i) carry'
   end
 
 val mont_reduction:
@@ -95,7 +115,7 @@ val mont_reduction:
 let mont_reduction #rLen rrLen n nInv_u64 c tmp res =
   let rLen2 = add #SIZE rrLen rrLen in
   copy rLen2 c tmp;
-  mont_reduction_ rrLen tmp n nInv_u64 (size 0);
+  mont_reduction_ rrLen tmp n nInv_u64 (size 0) (u64 0);
   //bn_rshift rLen2 tmp (mul #SIZE (size 64) rrLen) tmp; // tmp = tmp / r
   let tmp' = Buffer.sub #uint64 #(v rLen2) #rLen tmp rrLen rrLen in
   copy rrLen tmp' res
@@ -108,19 +128,22 @@ val to_mont:
   r2:lbignum rLen -> a:lbignum rLen -> 
   st_kara:lbignum (2 * rLen + 4 * v pow2_i) -> aM:lbignum rLen ->
   Stack unit
-    (requires (fun h -> live h n /\ live h r2 /\ live h a /\ live h aM /\ live h st_kara))
-    (ensures (fun h0 _ h1 -> preserves_live h0 h1))
+    (requires (fun h -> live h n /\ live h r2 /\ live h a /\ live h aM /\ live h st_kara /\
+                      disjoint st_kara a /\ disjoint st_kara r2 /\ disjoint st_kara n))
+    (ensures (fun h0 _ h1 -> preserves_live h0 h1 /\ modifies2 aM st_kara h0 h1))
   [@"c_inline"]
 let to_mont #rLen rrLen pow2_i iLen n nInv_u64 r2 a st_kara aM =
   let cLen = add #SIZE rrLen rrLen in
   let stLen = add #SIZE cLen (mul #SIZE (size 4) pow2_i) in
-  
   let c = Buffer.sub #uint64 #(v stLen) #(v cLen) st_kara (size 0) cLen in
-  let st_kara' = Buffer.sub #uint64 #(v stLen) #(4 * v pow2_i) st_kara cLen (mul #SIZE (size 4) pow2_i) in
-  assume (disjoint c a /\ disjoint c r2 /\ disjoint st_kara' a /\ disjoint st_kara' r2);
-  karatsuba #rLen pow2_i iLen rrLen a r2 st_kara' c; // c = a * r2
   assume (disjoint c n);
-  mont_reduction #rLen rrLen n nInv_u64 c c aM // aM = c % n
+ 
+  karatsuba #rLen pow2_i iLen rrLen a r2 st_kara; // c = a * r2
+  let h0 = FStar.HyperStack.ST.get() in
+  mont_reduction #rLen rrLen n nInv_u64 c c aM; // aM = c % n
+  let h1 = FStar.HyperStack.ST.get() in
+  assume (modifies2 aM st_kara h0 h1)
+
 
 val from_mont:
   #rLen:size_nat -> rrLen:size_t{v rrLen == rLen /\ rLen + rLen < max_size_t} ->
@@ -129,14 +152,14 @@ val from_mont:
   n:lbignum rLen -> nInv_u64:uint64 ->
   aM:lbignum rLen -> st:lbignum (rLen + rLen) -> a:lbignum rLen ->
   Stack unit
-    (requires (fun h -> live h n /\ live h a /\ live h aM /\ live h st))
-    (ensures (fun h0 _ h1 -> preserves_live h0 h1))
+    (requires (fun h -> live h n /\ live h a /\ live h aM /\ live h st /\ 
+                      disjoint st n))
+    (ensures (fun h0 _ h1 -> preserves_live h0 h1 /\ modifies2 a st h0 h1))
   [@"c_inline"]
 let from_mont #rLen rrLen pow2_i iLen n nInv_u64 aM st a =
   let rLen2 = add #SIZE rrLen rrLen in
   fill rLen2 st (u64 0);
-  let st' = Buffer.sub #uint64 #(v rLen2) #rLen st (size 0) rrLen in
+  let st' = Buffer.sub #uint64 #(v rLen2) #rLen st (size 0) rrLen in  
   copy rrLen aM st';
-  assume (disjoint st n);
   mont_reduction #rLen rrLen n nInv_u64 st st a // a = aM % n
 
